\listfiles
\documentclass{article}

\usepackage{amsmath}
\usepackage{amssymb}

\usepackage[a4paper,margin=1in]{geometry}

\setlength\parindent{0pt}

\title{18.014 pset 2}
\date{}

\begin{document}
\maketitle

\setcounter{section}{9}
\section{Show that we have the following equations for any $p,q$}

$h(0,p,q) = q+1
\\
h(1,p,q) = h(0,p,h(1,p,q-1)) = h(1,p,q-1) + 1 = ... = h(1,p,0) + q = p + q
\\
h(2,p,q) = h(1,p,h(2,p,q-1)) = p + h(2,p,q-1) = ... = pq
\\
h(3,p,q) = h(2,p,h(3,p,q-1)) = p*h(3,p,q-1) = ...p^q
\\
h(4,p,q) = h(3,p,h(4,p,q-1)) = p^{h(4,p,q-1)} = p^{p^{p^{...}}}$

\section{Compute explicitly...}

$h(4,2,4) = 2^{2^{2^2}} = 2^16 = 65536$
\\
$h(5,3,2) = h(4,3,h(5,3,1)) = h(4,3,h(4,3,h(5,3,0))) = h(4,3,h(4,3,1)) = h(4,3,3) = 3^{3^3} = 3^27 \approx 8 \times 10^{12}$

For $n>3$ we can prove

$h(n,2,1) = h(n-1,2,h(n,2,0)) = h(n-1,2,1) = 2$

and using this

$h(n,2,2) = h(n-1,2,h(n,2,1) = h(n-1,2,2)$

\section{Show that $a$ is injective}

$h(n,n,n-1) > n$
$h(n,n,n) = h(n-1,n,h(n,n,n-1)) > h(n-1,n-1,h(n,n,n-1)) > h(n-1,n-1,n-1)$

\section{For any natural...}

$a$ is injective

\end{document}
