\documentclass[letterpaper]{article}

\usepackage{geometry}
\usepackage{amsmath}
\usepackage{tikz}
\usepackage{pgfplots}
\usepackage{titlesec}


\setlength\parindent{0em}


\begin{document}

\section{Arithmetic and Geometric Progressions}
\section{Summation of Series}

\subsection{Sigma Notation}

\begin{align*}
\sum_{T=1}^n T_r = T_1 + T_2 + T_3 + \ldots + T_n
\end{align*}

Number of terms = $m - n + 1$

Express the following in sigma notation

\begin{enumerate}
\item $1 - \cfrac{1}{2} + \cfrac{1}{3} - \cfrac{1}{4} + \ldots$
\item $3 + 5 + 7 + 9 + ... + 41$
\item $1 \times 3 - 2 \times 5 + 3 \times 7 - 4 \times 9 + 5 \times 11$
\end{enumerate}

Write down the first 3 terms of the following sums

\begin{enumerate}
\item $\sum_{k=1}^{100} (3k - 1)$
\item $\sum_{k=1}^{40} (2 r^2)$
\item $\sum_{k=3}^{10} (r-1)(2r + 1)$
\end{enumerate}

\subsection{Basic Properties of Sigma}

\begin{align*}
\sum_{r=1}^n kT_r &= k\sum_{r=1}^n T_r \\
k\sum_{r=1}^n (T_r + G_r) &= \sum_{r=1}^n T_r + \sum_{r=1}^n G_r \\
\sum_{r=m}^n T_r &= \sum_{r=1}^n T_r - \sum_{r=1}^{m-1} T_r
\end{align*}

True or False?

\begin{enumerate}
\item $\sum_{r=1}^{100} (2r + 1) = \sum_{r=1}^{100} (2r) + 1$
\item $\sum_{n=1}^{100} (2n + 1) = \sum_{m=1}^{100} (2n + 1)$
\item $\sum_{n=1}^{100} a_n = \sum_{n=0}^{99} T_{n+1}$
\item $\sum_{m=1}^{100} m^2 = \sum_{m=0}^{100} m^2$
\item $\sum_{r=1}^{100} a = 100a$
\item $\sum_{n=1}^{100} (2n + 1) = \sum_{m=2}^{101} (2m - 1)$
\item $\sum_{m=1}^k (m + 2) = \sum_{m = 0}^k m + \sum_{m=0}^k 2$
\end{enumerate}

\subsection{Basic Formulas}

\begin{align*}
\sum_{r=1}^n r &= \cfrac{1}{2} n (n + 1) \\
\sum_{r=1}^n r^2 &= \cfrac{1}{6} n (2n + 1) \\
\sum_{r=1}^n r^3 &= \cfrac{1}{4} n^2 (n+1)^2
\end{align*}

Evaluate $\sum_{r=1}^n (r+2)(2r - 1)$ in terms of $n$.

Find $\sum_{k=0}^n (2n + 1 - 2k)$ in terms of $n$.

Find an expression, in simplified form, for $\sum_{r = n+1}^{2n} (2r - 1)^2$.

\subsection{Method of difference}

If a general term $T_r$ can be expressed as $G_{r+1} - G_r$, then

\begin{align*}
\sum_{r=1}^n T_r &= \sum_{r=1}^n (G_{r+1} - G_r) \\
&= G_n - G_0
\end{align*}

Evaluate $\sum_{r=1}^{100} \cfrac{1}{r(r+1)}$

Find the partial fractions of $\cfrac{1}{(2x - 1)(2x + 1))}$. Hence, find the sum of $\cfrac{1}{1 \times 3} + \cfrac{1}{3 \times 5} + \ldots + \cfrac{1}{(2n - 1)(2n + 1)}$

Express $\cfrac{2}{y(y+1)(y+2)}$ in partial fractions. Using this result, show that

\begin{align*}
\sum_{r=1}^N \cfrac{1}{r(r+1)(r+2)} = \cfrac{1}{4} - \cfrac{1}{2(N+1)(N+2)}
\end{align*}

By considering $\cfrac{1}{1 + a^{n-1}} - \cfrac{1}{1 + a^n}$ or otherwise, show that $\sum_{n=1}^N \cfrac{a^{n-1}}{(1 + a^{n-1})(1 + a^n)} = \cfrac{a^N - 1}{2(a-1)(a^N + 1)}$, where $a$ is positive and $a \neq 1$. Deduce that $\sum_{n=1}^N \cfrac{2^n}{(1 + 2^{n-1})(1 + 2^n)} < 1$.

Express $\cfrac{2}{n(n+1)(n+2)}$ in partial fractions. Hence, evaluate $\sum_{k=1}^{99} \cfrac{1}{k(k+1)(k+2)}$

Expand $n^2 - (n-1)^2 e$. Hence or otherwise, prove that $\sum_{n=1}^{N} e^n \left[(1-e)n^2 + 2ne - e\right] = N^2 e^N$.

Find $\sum_{r=2}^n \left[r - 2 -2n\left(\cfrac{1}{r-1} - \cfrac{1}{r}\right)\right]$ in terms of $n$.

Show that $\cfrac{1}{n^2 - n + 2} - \cfrac{1}{n^2 + n + 2} = \cfrac{2n}{n^4 + 3n^2 + 4}$. Find an expression in terms of $N$ for the sum $S_N$ where $S_N = \sum_{n=1}^N \cfrac{n}{n^4 + 3n^2 + 4}$. Deduce that $S_N < \cfrac{1}{4}$.
\end{document}
