\listfiles
\documentclass{article}

\usepackage{amsmath}
\usepackage{amssymb}

\usepackage[a4paper,margin=1in]{geometry}
\setlength{\parindent}{0in}
\setlength{\parskip}{1ex plus 0.5ex minus 0.2ex}
\newcommand{\sgn}{\operatorname{sgn}}
\newcommand{\mb}{\mathbf}

\title{ESN and Cartesian-Tensors}
\date{}

\begin{document}
\maketitle

\section{Introduction}

Consider vectors $\mb{a} = a_x\mb{x} + a_y\mb{y} + a_z\mb{z}$ and $\mb{b} = b_x\mb{x} + b_y\mb{y} + b_z\mb{z}$. If we wish to prove a simple theorem like the fact that $\frac{d}{dt} (\mb{a} \cdot \mb{b}) = \mb{a} \cdot \frac{d\mb{b}}{dt} + \mb{b} \cdot \frac{d\mb{a}}{dt}$ we'll have to write the following long proof

\begin{align}
\mb{a} \cdot \mb{b} &= a_x b_x + a_y b_y + a_z b_z \\
\frac{d}{dt} (\mb{a} \cdot \mb{b}) &= \frac{d}{dt}(a_x b_x + a_y b_y + a_z b_z) \\
&= \frac{d}{dt}(a_x b_x) + \frac{d}{dt}(a_y b_y) + \frac{d}{dt}(a_z b_z) \\
&= (\frac{d}{dt}a_x) b_x + a_x (\frac{d}{dt}b_x) + (\frac{d}{dt}a_y) b_y + a_y (\frac{d}{dt}b_y) + ... \\
&= a_x (\frac{d}{dt}b_x) + a_y (\frac{d}{dt}b_y) + ... \\
&\ + (\frac{d}{dt}a_x) b_x + (\frac{d}{dt}a_y) b_y + ... \\
&= \mb{a} \cdot \frac{d\mb{b}}{dt} + \mb{b} \cdot \frac{d\mb{a}}{dt}
\end{align}

a tedious manipulation of components. We introduce ESN by the two rules:

\begin{enumerate}
\item{indiced run over all possible values they can take}
\item{repeated indices are implicitly summed over}
\end{enumerate}

so in ESN

\begin{align}
\mb{a} \cdot \mb{b} &= a_i b_i \\
&= \sum_{i=1,2,3} a_i b_i
\end{align}

Normally we index our vectors by numbers instead of letters. 

\section{Orthogonal transformations preserve length}

\begin{align}
a_i &= M_{ij}b_j \\
a_i a_i &= M_{ij}b_j M_{ij'}b_{j'} \\
&= M_{ij}M_{ij'} b_jb_{j'} \\
&= \delta_{jj'} b_jb_{j'} \\
&= b_jb_j
\end{align}

The first line may be writwen as $a = M_{\_j} b_j$, showing that $a$ is a linear combination of columns of $M (M_{\_j})$ with the entries of $b (b_j)$ as coefficients.

\section{Cartesian-tensors}

\begin{align}
T' &= aTa^{-1} \\
[aT]_{il} &= a_{ik}T_{kl} \\
[aTa^{-1}]_{ij} &= [aT]_{il} a^{-1}_{lj} \\
&= a_{ik}T_{kl}a_{jl}
\end{align}

$a_{ik}T_{kl} = a_{i\_} T_{\_l}$

\section{Very useful identity}
$\epsilon_{ijk}\epsilon_{klm} = \delta_{il}\delta_{jm} - \delta_{jl}\delta_{im}$

\end{document}
